verif/btrees/verif_splitnode_part3.v
@@ -1,0 +1,491 @@
+(** * verif_splitnode.v : Correctness proof of splitnode *)
+
+Require Import VST.floyd.proofauto.
+Require Import VST.floyd.library.
+Require Import relation_mem.
+Instance CompSpecs : compspecs. make_compspecs prog. Defined.
+Definition Vprog : varspecs. mk_varspecs prog. Defined.
+
+Require Import VST.msl.wand_frame.
+Require Import VST.msl.iter_sepcon.
+Require Import VST.floyd.reassoc_seq.
+Require Import VST.floyd.field_at_wand.
+Require Import FunInd.
+Require Import btrees.
+Require Import btrees_sep.
+Require Import btrees_spec.
+Require Import verif_newnode.
+Require Import verif_findindex.
+Require Import index.
+Require Import verif_splitnode_part0.
+
+Opaque Znth.
+
+Lemma integrity_intern_insert: forall X (le:listentry X) k c i e n0,
+  (* This can't be right, there must be more constraints on n0 *)
+    intern_le le (@node_depth X n0)->
+    nth_entry_le i (insert_le le (keychild X k c)) = Some e ->
+    exists ki ci, e = keychild X ki ci.
+Proof.
+Admitted. 
+
+Definition splitnode_main_if_else_part2 : statement :=
+ ltac:(let x := constr:(splitnode_main_if_else) in
+         let x := eval hnf in x in
+         match x with context [Ssequence (Sassign   (Efield
+                          (Ederef
+                            (Etempvar _node (tptr (Tstruct _BtNode noattr)))
+                            (Tstruct _BtNode noattr)) _numKeys tint)
+                        (Econst_int (Int.repr ?M) tint)) ?S] =>
+          exact (Ssequence (Sassign   (Efield
+                          (Ederef
+                            (Etempvar _node (tptr (Tstruct _BtNode noattr)))
+                            (Tstruct _BtNode noattr)) _numKeys tint)
+                        (Econst_int (Int.repr M) tint)) S)
+         end).
+
+Lemma splitnode_main_ifelse_part2_proof:
+ forall (Espec : OracleKind) (ptr0 : option (node val))
+     (le : listentry val) (First Last : bool) (nval pe : val) 
+     (gv : globals) (v_allEntries : val) (ke : key) (ce : node val)
+    (LEAFENTRY : LeafEntry (keychild val ke ce) =
+            LeafNode (btnode val ptr0 le false First Last nval)),
+   let n := btnode val ptr0 le false First Last nval : node val in 
+   forall (H0 : numKeys n = Fanout)
+      (H : node_integrity (btnode val ptr0 le false First Last nval)) 
+      (k : key) (fri : nat) 
+      (HFRI : findRecordIndex n k = ip fri)
+      (INRANGE : 0 <= idx_to_Z (ip fri) <= Z.of_nat Fanout) 
+      (vnewnode : val)
+      (H1 : vnewnode <> nullval)
+     (nleft := btnode val ptr0 le false First false nval : node val)
+     (PTRCE : isptr (getval ce))
+     (allent_end : list (val * (val + val)))
+    (H3 : Datatypes.length allent_end =
+     (Fanout + 1 - Z.to_nat (Z.of_nat fri))%nat)
+     (FRIRANGE : (0 <= fri < 16)%nat)
+     (H5 : key_repr ke = key_repr k)
+     (H4 : 0 <= Z.of_nat fri <
+        Zlength
+           (le_to_list (nth_first_le le (Z.to_nat (Z.of_nat fri))) ++
+             allent_end))
+     (FRILENGTH : Zlength
+              (le_to_list (nth_first_le le (Z.to_nat (Z.of_nat fri)))) =
+            Z.of_nat fri),
+
+semax (func_tycontext f_splitnode Vprog Gprog [])
+  (EX ent_end : list (val * (val + val)),
+   PROP (Z.of_nat fri <= Z.of_nat Fanout <= Z.of_nat Fanout;
+   Datatypes.length ent_end = (Fanout - Z.to_nat (Z.of_nat Fanout))%nat)
+   LOCAL (temp _i (Vint (Int.repr (Z.of_nat Fanout)));
+   temp _newNode vnewnode; temp _tgtIdx (Vint (Int.repr (Z.of_nat fri)));
+   lvar _allEntries (tarray tentry 16) v_allEntries; 
+   temp _node nval; temp _entry pe)
+   SEP (mem_mgr gv; btnode_rep nleft;
+   btnode_rep (empty_node false false Last vnewnode);
+   data_at Ews tentry (Vint (Int.repr (k_ k)), inl (getval ce)) pe;
+   data_at Tsh (tarray tentry 16)
+     (le_to_list (nth_first_le le (Z.to_nat (Z.of_nat fri))) ++
+      (Vint (Int.repr (k_ k)), inl (getval ce))
+      :: le_to_list (suble fri (Z.to_nat (Z.of_nat Fanout)) le) ++ ent_end)
+     v_allEntries; entry_rep (keychild val ke ce)))
+  splitnode_main_if_else_part2
+  (frame_ret_assert
+     (function_body_ret_assert tvoid
+        (EX newx : val,
+         PROP ( )
+         LOCAL ()
+         SEP (mem_mgr gv;
+         btnode_rep
+           (splitnode_left (btnode val ptr0 le false First Last nval)
+              (keychild val ke ce));
+         entry_rep
+           (splitnode_right (btnode val ptr0 le false First Last nval)
+              (keychild val ke ce) newx);
+         data_at Ews tentry
+           (key_repr
+              (splitnode_key (btnode val ptr0 le false First Last nval)
+                 (keychild val ke ce)), inl newx) pe))%assert)
+     (stackframe_of f_splitnode)).
+Proof.
+    intros. pose proof I.
+    unfold splitnode_main_if_else_part2.
+    abbreviate_semax.
+    Intros ent_end.
+    deadvars!.
+    pose (e:=keychild val ke ce).
+    rewrite unfold_btnode_rep with (n:=nleft).
+    unfold nleft. Intros ent_end0.
+    forward.                    (* node->numKeys=8 *)
+    gather_SEP (le_iter_sepcon le) (entry_rep (keychild val ke ce)).
+    replace_SEP 0 (le_iter_sepcon (insert_le le e)).
+    { entailer!. rewrite <- insert_rep. simpl. entailer!. }
+    rewrite le_split with (le0:=insert_le le e) (i:=Middle) by
+        (simpl in H0; rewrite numKeys_le_insert; rewrite H0; rewrite Middle_eq; rewrite Fanout_eq; omega).
+    rewrite le_iter_sepcon_app.
+    
+    forward_if (PROP ( )
+    LOCAL (temp _newNode vnewnode; temp _tgtIdx (Vint (Int.repr (Z.of_nat fri)));
+           lvar _allEntries (tarray tentry 16) v_allEntries; temp _node nval; temp _entry pe)
+    SEP (mem_mgr gv; btnode_rep (splitnode_left n e); btnode_rep (empty_node false false Last vnewnode);
+         data_at Ews tentry (Vint (Int.repr (k_ k)), inl (getval ce)) pe;
+         data_at Tsh (tarray tentry 16) (le_to_list (nth_first_le le (Z.to_nat (Z.of_nat fri))) ++ (Vint (Int.repr (k_ k)), inl (getval ce)) :: le_to_list (suble (fri) ((Z.to_nat (Z.of_nat Fanout))) le) ++ ent_end) v_allEntries; le_iter_sepcon (skipn_le (insert_le le e) Middle))).
+    {                           (* fri < 8 *)
+      Intros.
+      unfold Sfor.              (* both forward_loop and forward_for_simple_bound fail here *)
+      forward.                  (* i=tgtIdx *)
+      forward_loop (EX i:Z, EX le_end:list(val*(val+val)), PROP(Z.of_nat fri <= i <= Z.of_nat Middle)
+LOCAL (temp _newNode vnewnode; temp _tgtIdx (Vint (Int.repr (Z.of_nat fri)));
+       lvar _allEntries (tarray tentry 16) v_allEntries; temp _node nval; temp _entry pe;
+      temp _i (Vint (Int.repr i)))
+SEP (mem_mgr gv; le_iter_sepcon (nth_first_le (insert_le le e) Middle);
+          le_iter_sepcon (skipn_le (insert_le le e) Middle); malloc_token Ews tbtnode nval;
+     data_at Ews tbtnode
+       (Val.of_bool false,
+       (Val.of_bool First,
+       (Val.of_bool false,
+       (Vint (Int.repr 8),
+       (match ptr0 with
+        | Some n' => getval n'
+        | None => nullval
+        end, le_to_list (nth_first_le (insert_le le e) (Z.to_nat i)) ++ le_end))))) nval;
+     match ptr0 with
+     | Some n' => btnode_rep n'
+     | None => emp
+     end; btnode_rep (empty_node false false Last vnewnode);
+     data_at Ews tentry (Vint (Int.repr (k_ k)), inl (getval ce)) pe;
+     data_at Tsh (tarray tentry 16)
+       (le_to_list (nth_first_le le (Z.to_nat (Z.of_nat fri))) ++
+        (Vint (Int.repr (k_ k)), inl (getval ce))
+        :: le_to_list (suble fri (Z.to_nat (Z.of_nat Fanout)) le) ++ ent_end) v_allEntries))%assert.
+      - Exists (Z.of_nat fri).
+        Exists (le_to_list(skipn_le le fri) ++ ent_end0).
+        entailer!.
+        { split. omega.  rewrite Middle_eq. simpl. omega. }
+        rewrite le_split with (i:=fri) (le0:=le) at 1.
+        rewrite le_to_list_app.
+        rewrite Nat2Z.id. 
+        replace (nth_first_le (insert_le le e) fri) with (nth_first_le le fri).
+        rewrite app_assoc. cancel. apply derives_refl.
+        rewrite insert_fri with (fri:=fri) (key0:=ke).
+        rewrite nth_first_app_same1. auto.
+        rewrite numKeys_nth_first. auto.
+        simpl in H0. rewrite H0. omega. unfold e. simpl. auto.
+        simpl in HFRI. rewrite <- HFRI. apply FRI_repr. auto.
+        simpl in H0. rewrite H0. omega.
+      -                         (* loop body *)
+        Intros i.
+        Intros le_end.             
+        forward_if.
+        + assert(HINSERT: (le_to_list (nth_first_le le (Z.to_nat (Z.of_nat fri))) ++ (Vint (Int.repr (k_ k)), inl (getval ce)) :: le_to_list (suble (fri) ((Z.to_nat (Z.of_nat Fanout))) le) ++ ent_end) = le_to_list (insert_le le e) ++ ent_end).
+          { rewrite insert_fri with (fri:=fri) (key0:=ke).
+            rewrite le_to_list_app.
+            simpl. rewrite Nat2Z.id. rewrite H5. rewrite Nat2Z.id.
+            rewrite suble_skip. unfold key_repr.
+            rewrite <- app_assoc. auto.
+            unfold n in H0. simpl in H0. auto.      
+            unfold e. simpl. auto. unfold findRecordIndex in HFRI. unfold n in HFRI.
+            rewrite FRI_repr with (key2:=k) by auto. rewrite HFRI. auto.
+          } 
+          rewrite HINSERT.
+          assert(HENTRY: exists ei, nth_entry_le (Z.to_nat i) (insert_le le e) = Some ei).
+          { apply nth_entry_le_in_range. simpl in H0. rewrite numKeys_le_insert. rewrite H0.
+            rewrite Fanout_eq. rewrite Middle_eq in H9.
+            destruct H9. apply Z2Nat.inj_le in H11. rewrite Nat2Z.id in H11.
+            omega. omega. omega. }
+          destruct HENTRY as [ei HENTRY].  
+          assert (HEI: exists ki ci, ei = keychild val ki ci).
+          {simpl in H. destruct ptr0; try contradiction.
+           eapply integrity_intern_insert; eassumption. }
+          destruct HEI as [ki [ci HEI]]. subst ei.
+          assert_PROP(isptr (getval ci)).
+          { apply le_iter_sepcon_split in HENTRY.
+            gather_SEP (le_iter_sepcon (nth_first_le (insert_le le e) Middle))
+                       (le_iter_sepcon (skipn_le (insert_le le e) Middle)).
+            replace_SEP 0 (le_iter_sepcon (insert_le le e)).
+            { entailer!. rewrite le_split with (i:=Middle) (le0:= (insert_le le e)) at 3.
+              rewrite le_iter_sepcon_app. entailer!. simpl in H0. rewrite numKeys_le_insert.
+              rewrite H0. rewrite Middle_eq. rewrite Fanout_eq. omega. }
+            rewrite HENTRY. simpl entry_rep. entailer!. }
+          rename H11 into CIPTR.
+          assert(HZNTH: forall ent_end, Znth (d:=(Vundef,inl Vundef)) i (le_to_list (insert_le le e) ++ ent_end) = entry_val_rep (keychild val ki ci)).
+          { intros. rewrite <- Z2Nat.id with (n:=i). apply Znth_to_list. auto. omega. }
+          assert(0 <= i < 8).
+          { split. omega. rewrite Int.signed_repr in H10. auto.
+            rewrite Middle_eq in H9. simpl in H9. rep_omega. }
+          assert_PROP(Zlength le_end > 0).
+          { entailer!.
+            clear - H14 H11 H0. simplify_value_fits in H14.
+            destruct H14, H1, H2, H3, H4.
+            simplify_value_fits in H5. destruct H5.
+            rewrite Zlength_app in H5. rewrite le_to_list_length in H5.
+            rewrite numKeys_nth_first in H5. rewrite Z2Nat.id in H5. omega. omega.
+            simpl in H0. rewrite numKeys_le_insert. rewrite H0. rewrite Fanout_eq.
+            destruct H11. rewrite Z2Nat.inj_lt in H8. simpl in H8. omega. omega. omega. }            
+          rename H12 into LEEND.
+          forward.              (* t'20=allEntries[i]->key *)
+          { rewrite HZNTH. entailer!. }
+          rewrite HZNTH.
+          forward.              (* node->entries[i]->key=t'20 *)
+          forward.              (* t'19=allEntries[i]->ptr.record *)
+          { rewrite HZNTH. entailer!. }
+          rewrite HZNTH.
+          forward.              (* node->entries[i]->ptr.record = t'19 *)
+          forward.              (* i=i+1 *)
+          Exists (i+1).
+          Exists (sublist 1 (Zlength le_end) le_end). entailer!.
+          { rewrite Middle_eq. simpl. omega. }
+          
+          rewrite upd_Znth_twice.
+          rewrite upd_Znth_same.
+          rewrite upd_Znth_app2.
+          rewrite le_to_list_length.
+          rewrite numKeys_nth_first.
+          rewrite Z2Nat.id. replace(i-i) with 0 by omega.
+          rewrite upd_Znth0. replace (Z.to_nat (i+1)) with (S (Z.to_nat i)).
+          rewrite nth_first_increase with (e:=(keychild val ki ci)).
+          rewrite le_to_list_app. simpl. rewrite <- app_assoc.
+          cancel.
+          (* rewrite insert_fri with (fri:=fri) at 1. rewrite le_to_list_app. simpl. *)
+          (* rewrite Nat2Z.id. unfold suble. *)
+          (* rewrite Nat2Z.id. *)
+          (* rewrite nth_first_same with (m:=(Fanout - fri)%nat). *)
+          (* rewrite <- app_assoc. simpl. rewrite H5. unfold key_repr. cancel. *)
+          (* rewrite numKeys_le_skipn. simpl in H0. rewrite H0. auto. *)
+          (* auto. rewrite <- HFRI. simpl. apply FRI_repr. auto. *)
+          rewrite numKeys_le_insert. simpl in H0. rewrite H0. destruct H11.
+          rewrite Z2Nat.inj_lt in H22. simpl in H22. rewrite Fanout_eq. omega.
+          omega. omega.
+          auto.
+          rewrite Z2Nat.inj_add. simpl. omega. omega. omega. omega.
+          rewrite numKeys_le_insert. simpl in H0. rewrite H0. destruct H11.
+          rewrite Z2Nat.inj_lt in H22. simpl in H22. rewrite Fanout_eq. omega.
+          omega. omega.
+          rewrite le_to_list_length. rewrite numKeys_nth_first. rewrite Z2Nat.id.
+          rep_omega. omega.
+          rewrite numKeys_le_insert. simpl in H0. rewrite H0. destruct H11.
+          rewrite Z2Nat.inj_lt in H22. simpl in H22. rewrite Fanout_eq. omega.
+          omega. omega.
+          rewrite Zlength_app. rewrite le_to_list_length. rewrite numKeys_nth_first.
+          rewrite Z2Nat.id. split. omega. omega. omega.
+          rewrite numKeys_le_insert. simpl in H0. rewrite H0. destruct H11.
+          rewrite Z2Nat.inj_lt in H22. simpl in H22. rewrite Fanout_eq. omega.
+          omega. omega.
+          rewrite Zlength_app. rewrite le_to_list_length. rewrite numKeys_nth_first.
+          rewrite Z2Nat.id. split. omega. omega. omega.
+          rewrite numKeys_le_insert. simpl in H0. rewrite H0. destruct H11.
+          rewrite Z2Nat.inj_lt in H22. simpl in H22. rewrite Fanout_eq. omega.
+          omega. omega.
+        + rewrite Middle_eq in H9. simpl in H9. rewrite Int.signed_repr in H10 by rep_omega.
+          assert(i=8) by omega.
+          forward.              (* break *)
+          entailer!. unfold n, splitnode_left.
+          rewrite unfold_btnode_rep with (n:=btnode val ptr0 (nth_first_le (insert_le le e) Middle) false First false nval).
+          Exists le_end.
+          cancel. Opaque nth_first_le. simpl.
+          rewrite numKeys_nth_first. rewrite Middle_eq. simpl. cancel.
+          apply derives_refl.
+          simpl in H0. rewrite numKeys_le_insert. rewrite H0.
+          rewrite Middle_eq. rewrite Fanout_eq. omega.
+    } 
+    {                           (* fri >= 8 *)
+      forward.                  (* skip *)
+      entailer!.
+      assert((Middle <=? fri)%nat = true).
+      { clear -H8. rewrite Middle_eq. apply leb_correct.
+        assert(8 <= Z.of_nat fri) by omega. apply Z2Nat.inj_le in H. simpl in H.
+        rewrite Nat2Z.id in H. auto. omega. omega. }
+      unfold splitnode_left, n.
+      rewrite unfold_btnode_rep with (n:=btnode val ptr0 (nth_first_le (insert_le le e) Middle) false First false nval).
+      assert(SPLITLE: le_to_list le = le_to_list (nth_first_le le Middle) ++ le_to_list (skipn_le le Middle)).
+      { rewrite le_split with (i:=Middle) at 1. rewrite le_to_list_app. auto.
+        simpl in H0. rewrite H0. rewrite Middle_eq, Fanout_eq. omega. }
+      rewrite SPLITLE.
+      rewrite <- app_assoc.
+      Exists (le_to_list (skipn_le le Middle) ++ ent_end0).
+      simpl. rewrite numKeys_nth_first.
+      rewrite nth_first_insert with (k:=ke). cancel.
+      unfold e. simpl. auto. simpl in HFRI.
+      rewrite FRI_repr with (key2:=k). rewrite HFRI. simpl. rewrite Middle_eq. simpl. omega.
+      auto. simpl in H0. rewrite numKeys_le_insert. rewrite H0. rewrite Middle_eq.
+      rewrite Fanout_eq. omega.
+    }
+    rewrite unfold_btnode_rep with (n:=empty_node false false Last vnewnode).
+    simpl. Intros ent_empty.
+    assert(HINSERT: (le_to_list (nth_first_le le (Z.to_nat (Z.of_nat fri))) ++ (Vint (Int.repr (k_ k)), inl (getval ce)) :: le_to_list (suble (fri) ((Z.to_nat (Z.of_nat Fanout))) le) ++ ent_end) = le_to_list (insert_le le e) ++ ent_end).
+    { rewrite insert_fri with (fri:=fri) (key0:=ke).
+      rewrite le_to_list_app.
+      simpl. rewrite Nat2Z.id. rewrite H5. rewrite Nat2Z.id.
+      rewrite suble_skip. unfold key_repr.
+      unfold n in H0. simpl in H0. rewrite <- app_assoc. simpl. reflexivity.
+      simpl in H0. rewrite H0. auto.
+      unfold e. simpl. auto. unfold findRecordIndex in HFRI. unfold n in HFRI. 
+      rewrite FRI_repr with (key2:=k) by auto. rewrite HFRI. auto.
+    } 
+    rewrite HINSERT.
+    
+    forward_for_simple_bound (Z.of_nat (Fanout) + 1)
+(EX i:Z, EX ent_right:list(val*(val+val)),
+(PROP (Zlength ent_right + i - 9 = Z.of_nat Fanout; 9 <= i <= 16)
+     LOCAL (temp _newNode vnewnode; temp _tgtIdx (Vint (Int.repr (Z.of_nat fri)));
+     lvar _allEntries (tarray tentry 16) v_allEntries; temp _node nval; temp _entry pe)
+     SEP (mem_mgr gv; btnode_rep (splitnode_left n e);
+     malloc_token Ews tbtnode vnewnode;
+     data_at Ews tbtnode
+       (Vfalse, (Vfalse, (Val.of_bool Last, (Vint (Int.repr 0), (nullval, le_to_list(suble (S Middle) (Z.to_nat i) (insert_le le e)) ++ ent_right))))) vnewnode;
+     data_at Ews tentry (Vint (Int.repr (k_ k)), inl (getval ce)) pe;
+     data_at Tsh (tarray tentry 16) (le_to_list (insert_le le e) ++ ent_end) v_allEntries;
+     le_iter_sepcon (skipn_le (insert_le le e) Middle))))%assert.                             
+    
+    { rewrite Fanout_eq. simpl. rep_omega. }
+    { abbreviate_semax.
+      forward.                  (* i=9 *)
+      Exists 9. Exists ent_empty. entailer!.
+      split. rewrite Fanout_eq. simpl. rep_omega.
+      rewrite Fanout_eq. simpl.
+      simplify_value_fits in H11. destruct H11, H17, H18, H19, H20.
+      clear - H21. assert (value_fits (tarray tentry 15) ent_empty). auto.
+      simplify_value_fits in H. destruct H.
+      replace (Zlength ent_empty + 9 - 9) with (Zlength ent_empty) by omega.
+      auto.
+      apply derives_refl. }
+    {                           (* loop body *)
+      Intros.
+      assert(HENTRY: exists ei, nth_entry_le (Z.to_nat i) (insert_le le e) = Some ei).
+      { apply nth_entry_le_in_range. simpl in H0. rewrite numKeys_le_insert. rewrite H0.
+        rewrite Fanout_eq in H8. simpl in H8. rewrite Fanout_eq. destruct H8.
+        apply Z2Nat.inj_lt in H11. simpl in H11. auto. omega. omega. }
+      destruct HENTRY as [ei HENTRY].  
+      assert (HEI: exists ki ci, ei = keychild val ki ci).
+      { simpl in H; destruct ptr0; try contradiction.
+        eapply integrity_intern_insert; eassumption.  }
+      destruct HEI as [ki [ci HEI]]. subst ei.
+      assert_PROP(isptr (getval ci)).
+      { apply le_iter_sepcon_split in HENTRY.
+        rewrite unfold_btnode_rep with (n:=splitnode_left n e).
+        unfold splitnode_left. unfold n. Intros ent_left.
+        gather_SEP (le_iter_sepcon (nth_first_le (insert_le le e) Middle)) (le_iter_sepcon (skipn_le (insert_le le e) Middle)).
+        replace_SEP 0 ( le_iter_sepcon (insert_le le e)).
+        { entailer!. rewrite le_split with (i:=Middle) (le0:= (insert_le le e)) at 3.
+          rewrite le_iter_sepcon_app. entailer!. simpl in H0. rewrite numKeys_le_insert.
+          rewrite H0. rewrite Middle_eq. rewrite Fanout_eq. omega. }
+        rewrite HENTRY. simpl entry_rep. entailer!. }
+      rename H9 into CIPTR.
+      assert(HZNTH: forall ent_end, Znth (d:=(Vundef,inl Vundef)) i (le_to_list (insert_le le e) ++ ent_end) = entry_val_rep (keychild val ki ci)).
+      { intros. rewrite <- Z2Nat.id with (n:=i). apply Znth_to_list. auto. omega. }
+
+      rewrite Fanout_eq in H8. simpl in H8.
+      forward.                  (* t'18=allEntries[i]->key *)
+      { rewrite HZNTH. entailer!. }
+      rewrite HZNTH. simpl.
+      forward.                  (* newnode->entries[i-8]->key=t'18 *)
+      forward.                  (* t'17=allEntries[i]->ptr.record *)
+      { rewrite HZNTH. entailer!. }
+      rewrite HZNTH. simpl.
+      forward.                  (* newnode->entries[i-8]->ptr.record=t'17 *)
+      entailer!.
+      rename ent_right into x.
+      rewrite Fanout_eq in CIPTR. simpl in CIPTR. assert(Zlength x = 24 - i) by omega.
+      Exists (sublist 1 (Zlength x) x). entailer!.
+      { rewrite Fanout_eq. simpl. 
+        rewrite Zlength_sublist. omega. omega. omega. }
+      assert(9 <= Z.to_nat i < 16)%nat.
+      { clear - H10 H8. assert(HH: 9 <= i <= 16) by auto.
+        destruct H10. apply Z2Nat.inj_le in H0. apply Z2Nat.inj_le in H.
+        destruct H8. apply Z2Nat.inj_lt in H2.
+        simpl in H, H0, H1, H2. split. omega. omega. omega. omega. omega. omega. omega. omega. }
+      
+      rewrite upd_Znth_twice.
+      rewrite upd_Znth_same.
+      rewrite upd_Znth_app2.
+      rewrite le_to_list_length.
+      rewrite numKeys_suble.
+      rewrite Nat2Z.inj_sub.
+      rewrite Z2Nat.id. rewrite Middle_eq.
+      simpl. replace (i - 9 - (i - 9)) with 0 by omega.
+      rewrite upd_Znth0. replace (Z.to_nat (i+1)) with (S (Z.to_nat i)).
+      rewrite suble_increase with (e:=(keychild val ki ci)).
+      rewrite le_to_list_app. simpl. rewrite <- app_assoc.
+      cancel.
+       
+      rewrite numKeys_le_insert. simpl in H0. rewrite H0.
+      rewrite Fanout_eq. omega. auto.      
+      rewrite Z2Nat.inj_add. simpl. omega. omega. omega.
+      omega.
+      rewrite Middle_eq. omega.
+      rewrite numKeys_le_insert. simpl in H0. rewrite H0. rewrite Middle_eq. rewrite Fanout_eq. omega.
+      rewrite le_to_list_length. rewrite numKeys_suble.
+      rewrite Middle_eq. rewrite Nat2Z.inj_sub. rewrite Z2Nat.id. simpl.
+      omega. omega. omega.
+      rewrite numKeys_le_insert. simpl in H0. rewrite H0.
+      rewrite Middle_eq. rewrite Fanout_eq. omega.
+      rewrite Zlength_app. rewrite le_to_list_length. rewrite numKeys_suble. rewrite H21.
+      rewrite Middle_eq. rep_omega. rewrite numKeys_le_insert. simpl in H0. rewrite H0.
+      rewrite Middle_eq. rewrite Fanout_eq. omega. 
+      rewrite Zlength_app. rewrite le_to_list_length. rewrite numKeys_suble. rewrite H21.
+      rewrite Middle_eq. rep_omega. rewrite numKeys_le_insert. simpl in H0. rewrite H0.
+      rewrite Middle_eq. rewrite Fanout_eq. omega.
+    }
+    Intros ent_right.
+    forward.                    (* newnode->numKeys=7 *)
+    assert(NTHENTRY: exists emid, nth_entry_le Middle (insert_le le e) = Some emid).
+    { apply nth_entry_le_in_range. unfold n in H0. simpl in H0. rewrite numKeys_le_insert.
+      rewrite H0. rewrite Middle_eq.
+      rewrite Fanout_eq. omega. }
+    destruct NTHENTRY as [emid NTHENTRY].
+    assert (HEMID: exists ki ci, emid = keychild val ki ci).
+    { simpl in H; destruct ptr0; try contradiction.
+      eapply integrity_intern_insert; eassumption. }
+    destruct HEMID as [ki [ci HEMID]].
+    assert_PROP(isptr (getval ci)).
+    { apply le_iter_sepcon_split in NTHENTRY.
+      rewrite unfold_btnode_rep with (n:=splitnode_left n e).
+      simpl (splitnode_left n e). destruct (btnode val ptr0 (nth_first_le (insert_le le e) Middle) false First false nval) eqn:HDES. Intros ent_end1. inv HDES.
+      gather_SEP (le_iter_sepcon (nth_first_le (insert_le le e) Middle)) (le_iter_sepcon (skipn_le (insert_le le e) Middle)).
+      replace_SEP 0 (le_iter_sepcon (insert_le le e)).
+      { entailer!. rewrite le_split with (i:=Middle) (le0:=insert_le le e) at 3.
+        rewrite le_iter_sepcon_app. entailer!.
+        simpl in H0. rewrite numKeys_le_insert. rewrite H0. rewrite Fanout_eq. rewrite Middle_eq.
+        omega. }
+      rewrite NTHENTRY. simpl entry_rep. entailer!. }
+    assert(HZNTH: nth_entry_le Middle (insert_le le e) = Some emid) by auto.
+    eapply Znth_to_list with (endle:=ent_end) in HZNTH.
+    rewrite Middle_eq in HZNTH. simpl in HZNTH.
+    forward.                    (* t'5=allEntries[8]->ptr.child *)
+     { entailer!. rewrite HZNTH.
+       simpl. apply isptr_is_pointer_or_null. auto. }
+     rewrite HZNTH. rewrite HEMID. simpl.
+     forward.                   (* nenode->ptr0=t'5 *)
+     rewrite skipn_increase with (n:=Middle) (e:=emid). simpl. Intros.
+     gather_SEP (malloc_token Ews tbtnode vnewnode)
+                (data_at Ews tbtnode _ vnewnode)
+                (entry_rep emid)
+                (le_iter_sepcon (skipn_le (insert_le le e) (S Middle))).
+     replace_SEP 0 (btnode_rep (splitnode_internnode le e vnewnode Last ci)).
+     { entailer!. rewrite unfold_btnode_rep with (n:=splitnode_internnode le e vnewnode Last ci).
+       simpl.
+       Exists ent_right.
+       replace(Z.to_nat (Z.of_nat Fanout + 1)) with (S Fanout).
+       rewrite numKeys_le_skipn. rewrite numKeys_le_insert. simpl in H0. rewrite H0.
+       assert(HSUB: suble (S Middle) (S Fanout) (insert_le le e) = skipn_le (insert_le le e) (S Middle)).
+       { apply suble_skip. rewrite numKeys_le_insert. unfold n in H0. simpl in H0. rewrite H0.
+         auto.  }
+       rewrite HSUB.
+       rewrite Fanout_eq. rewrite Middle_eq.
+      replace (Z.of_nat(16 - 9)) with 7 by (simpl; omega). cancel.
+      apply derives_refl.
+      rewrite Fanout_eq. simpl. auto. }
+     
+     forward.                    (* t'16=allEntries[8]->key *)
+     { entailer!. rewrite HZNTH. simpl. auto. }
+     rewrite HZNTH.
+     forward.                    (* entry->key=t'16 *)
+     forward.                    (* entry->ptr.child=newnode *)
+     forward.                    (* return *)
+     Exists vnewnode. fold e. simpl. rewrite NTHENTRY. entailer!.
+     simpl. apply derives_refl.
+     rewrite numKeys_le_insert. simpl in H0. rewrite H0. rewrite Fanout_eq. rewrite Middle_eq. omega.
+     auto.
+Qed.
+
+
