verif/btrees/verif_splitnode_part4.v
@@ -1,0 +1,382 @@
+(** * verif_splitnode.v : Correctness proof of splitnode *)
+
+Require Import VST.floyd.proofauto.
+Require Import VST.floyd.library.
+Require Import relation_mem.
+Instance CompSpecs : compspecs. make_compspecs prog. Defined.
+Definition Vprog : varspecs. mk_varspecs prog. Defined.
+
+Require Import VST.msl.wand_frame.
+Require Import VST.msl.iter_sepcon.
+Require Import VST.floyd.reassoc_seq.
+Require Import VST.floyd.field_at_wand.
+Require Import FunInd.
+Require Import btrees.
+Require Import btrees_sep.
+Require Import btrees_spec.
+Require Import verif_newnode.
+Require Import verif_findindex.
+Require Import index.
+Require Import verif_splitnode_part0.
+Require Import verif_splitnode_part3.
+
+Opaque Znth.
+
+Lemma splitnode_main_if_else_proof:
+ forall (Espec : OracleKind)
+   (ptr0 : option (node val))  (le : listentry val) (isLeaf First Last : bool)
+   (nval : val) (e : entry val) (pe : val) (gv : globals) (v_allEntries : val)
+  (H : node_integrity (btnode val ptr0 le isLeaf First Last nval)),
+  let n := btnode val ptr0 le isLeaf First Last nval : node val in
+  forall (H0 : numKeys n = Fanout)
+  (LEAFENTRY : LeafEntry e = LeafNode (btnode val ptr0 le isLeaf First Last nval))
+  (keyrepr : val) (coprepr : val + val)
+  (HEVR : entry_val_rep e = (keyrepr, coprepr))
+  (k : key) (HK : keyrepr = key_repr k)
+  (INRANGE : 0 <= idx_to_Z (findRecordIndex n k) <= Z.of_nat Fanout)
+  (vnewnode : val)
+  (H1 : vnewnode <> nullval)
+  (ent_end : list (val * (val + val)))
+  (H2 : typed_false tint
+       (force_val
+          (both_int
+             (fun n1 n2 : int => Some (Val.of_bool (Int.eq n1 n2)))
+             sem_cast_pointer sem_cast_pointer 
+             (Val.of_bool isLeaf) (Vint (Int.repr 1))))),
+
+semax (func_tycontext f_splitnode Vprog Gprog [])
+  (PROP ( )
+   LOCAL (temp _t'3 (Val.of_bool isLeaf); temp _newNode vnewnode;
+   temp _t'2 vnewnode; temp _t'27 (Val.of_bool Last);
+   temp _tgtIdx
+     (Vint (Int.repr (rep_index (findRecordIndex' le k (ip 0)))));
+   temp _t'1
+     (Vint (Int.repr (rep_index (findRecordIndex' le k (ip 0)))));
+   temp _t'28 keyrepr;
+   lvar _allEntries (tarray (Tstruct _Entry noattr) 16) v_allEntries;
+   temp _node nval; temp _entry pe;
+   temp _isLeaf (Val.of_bool isLeaf))
+   SEP (mem_mgr gv; @malloc_token btrees.CompSpecs Ews tbtnode nval;
+   data_at Ews tbtnode
+     (Val.of_bool isLeaf,
+     (Val.of_bool First,
+     (Vint (Int.repr 0),
+     (Vint
+        (Int.repr
+           (Z.of_nat
+              (numKeys (btnode val ptr0 le isLeaf First Last nval)))),
+     (match ptr0 with
+      | Some n' => getval n'
+      | None => nullval
+      end, le_to_list le ++ ent_end))))) nval;
+   match ptr0 with
+   | Some n' => btnode_rep n'
+   | None => emp
+   end; le_iter_sepcon le;
+   btnode_rep (empty_node isLeaf false Last vnewnode);
+   data_at_ Tsh (tarray (Tstruct _Entry noattr) 16) v_allEntries;
+   entry_rep e; data_at Ews tentry (keyrepr, coprepr) pe))
+  splitnode_main_if_else
+  (frame_ret_assert
+     (function_body_ret_assert tvoid
+        (EX newx : val,
+         PROP ( )
+         LOCAL ()
+         SEP (mem_mgr gv;
+         btnode_rep
+           (splitnode_left (btnode val ptr0 le isLeaf First Last nval)
+              e);
+         entry_rep
+           (splitnode_right
+              (btnode val ptr0 le isLeaf First Last nval) e newx);
+         data_at Ews tentry
+           (key_repr
+              (splitnode_key
+                 (btnode val ptr0 le isLeaf First Last nval) e),
+           inl newx) pe))%assert) (stackframe_of f_splitnode)).
+Proof.
+ intros.
+ abbreviate_semax.
+    assert(INTERN: isLeaf=false).
+    { destruct isLeaf; auto. simpl in H2. inv H2. }
+    destruct (findRecordIndex n k) as [|fri] eqn:HFRI.
+    { simpl in INRANGE. omega. }
+    replace (findRecordIndex' le k (index.ip 0)) with (index.ip fri). simpl.
+    gather_SEP (malloc_token Ews tbtnode nval)
+               (data_at Ews tbtnode _ nval)
+               (match ptr0 with
+                | Some n' => btnode_rep n'
+                | None => emp
+                end) (le_iter_sepcon le).
+    pose (nleft := btnode val ptr0 le false First false nval).
+    replace_SEP 0 (btnode_rep nleft).
+    { entailer!. rewrite unfold_btnode_rep with (n:=nleft). unfold nleft.
+      Exists ent_end. cancel. } clear ent_end. fold tentry.
+    assert(ENTRY: exists ke ce, e = keychild val ke ce). (* the entry to be inserted at an intern node must be keychild *)
+    { destruct e. simpl in LEAFENTRY.
+      rewrite INTERN in LEAFENTRY. exfalso. rewrite <- LEAFENTRY. auto. eauto. }
+    destruct ENTRY as [ke [ce ENTRY]].
+    assert_PROP(isptr (getval ce)).
+    { rewrite ENTRY. unfold entry_rep. entailer!. }
+    rename H3 into PTRCE.
+    
+    forward_for_simple_bound (Z.of_nat fri)
+    (EX i:Z, EX allent_end:list (val*(val+val)),
+     (PROP (length allent_end = (Fanout + 1 - Z.to_nat(i))%nat)
+      LOCAL (temp _t'3 (Val.of_bool isLeaf); temp _newNode vnewnode; temp _t'2 vnewnode;
+      temp _t'27 (Val.of_bool Last); temp _tgtIdx (Vint (Int.repr (Z.of_nat fri)));
+      temp _t'1 (Vint (Int.repr (Z.of_nat fri))); temp _t'28 keyrepr;
+      lvar _allEntries (tarray tentry 16) v_allEntries; temp _node nval; temp _entry pe;
+      temp _isLeaf (Val.of_bool isLeaf))
+      SEP (mem_mgr gv; btnode_rep nleft; btnode_rep (empty_node isLeaf false Last vnewnode);
+           data_at Tsh (tarray tentry 16) (le_to_list (nth_first_le le (Z.to_nat i))++ allent_end) v_allEntries; entry_rep e; data_at Ews tentry (keyrepr, coprepr) pe)))%assert.
+    { simpl in INRANGE. rewrite Fanout_eq in INRANGE.
+      replace (Z.of_nat 15) with 15 in INRANGE. rep_omega. simpl. auto. }
+    { entailer!.
+      Exists (default_val (nested_field_type (tarray (Tstruct _Entry noattr) 16) [])).
+      entailer!. unfold data_at_, field_at_. entailer!. }
+    {                           (* loop body *)
+      rewrite unfold_btnode_rep with (n:=nleft). unfold nleft.
+      Intros ent_end.
+      assert(HENTRY: exists e, nth_entry_le (Z.to_nat i) le = Some e).
+      { apply nth_entry_le_in_range. simpl in INRANGE. rewrite Fanout_eq in INRANGE.
+        unfold n in H0. simpl in H0. rewrite H0. rewrite Fanout_eq. apply Nat2Z.inj_lt.
+        simpl. rewrite Z2Nat.id. simpl in INRANGE. omega. omega. }
+      destruct HENTRY as [ei HENTRY].
+      assert (HEI: exists ki ci, ei = keychild val ki ci).
+      { eapply integrity_nth. eauto. rewrite INTERN. simpl. auto. eauto. }
+      destruct HEI as [ki [ci HEI]]. subst ei.
+      assert_PROP(isptr (getval ci)).
+      { apply le_iter_sepcon_split in HENTRY. rewrite HENTRY. simpl entry_rep. entailer!. }
+      rename H5 into CIPTR.
+      assert(HZNTH: forall ent_end, Znth (d:=(Vundef,inl Vundef)) i (le_to_list le ++ ent_end) = entry_val_rep (keychild val ki ci)).
+      { intros. rewrite <- Z2Nat.id with (n:=i). apply Znth_to_list. auto. omega. }
+      assert(HIRANGE: (0 <= i < 15)).
+      { clear -INRANGE H3. simpl in INRANGE. rewrite Fanout_eq in INRANGE.
+        replace (Z.of_nat 15) with 15 in INRANGE by auto. omega. }  
+      forward.                  (* t'26 = node->entries[i].key *) 
+      { entailer!. rewrite HZNTH. simpl; auto. }
+      rewrite HZNTH. simpl.
+      Opaque Znth.
+      forward.                 (* allEntries[i].key = t'26 *)
+      forward.                 (* t'25=node->entries[i]->ptr.record *)
+      { rewrite HZNTH. entailer!. }
+      rewrite HZNTH. simpl.
+      forward.                  (* allEntries[i]->ptr.record=t'25 *)
+      entailer!.
+      rename allent_end into x.
+      assert(XEMP: Zlength x > 0).
+      { destruct x. clear - H4 HIRANGE. simpl in H4. rewrite Fanout_eq in H4.
+        apply eq_sym in H4. apply NPeano.Nat.sub_0_le in H4. apply inj_le in H4.
+        replace (Z.of_nat (15 + 1)) with 16 in H4. rewrite Z2Nat.id in H4. rep_omega.
+        omega. simpl. auto.
+        rewrite Zlength_cons. rep_omega. }
+      Exists (sublist 1 (Zlength x) x). entailer!.
+      { clear -H4 H3 XEMP.
+        destruct x.
+        - rewrite Zlength_nil in XEMP. omega.
+        - rewrite sublist_1_cons. rewrite Zlength_cons. rewrite Zsuccminusone.
+          rewrite sublist_same by omega. simpl in H4. rewrite Z2Nat.inj_add by omega.
+          simpl.
+          assert((Fanout + 1 - Z.to_nat i)%nat = S(Fanout + 1 - (Z.to_nat i + 1))) by omega.
+          rewrite H in H4. inv H4. omega. }
+      assert(INUM: (Z.to_nat i <= numKeys_le le)%nat).
+      { unfold n  in H0. simpl in H0. rewrite H0. clear -INRANGE H3.
+        simpl in INRANGE. apply Nat2Z.inj_le.
+        simpl. rewrite Z2Nat.id. simpl in INRANGE. omega. omega. }
+      rewrite unfold_btnode_rep with (n:=nleft). unfold nleft. Exists ent_end. cancel.      
+      rewrite upd_Znth_twice.
+      rewrite app_Znth2. rewrite le_to_list_length. rewrite numKeys_nth_first. rewrite Z2Nat.id.
+      replace (i-i) with 0 by omega.
+      rewrite upd_Znth_app2.
+      rewrite le_to_list_length. rewrite numKeys_nth_first. rewrite Z2Nat.id.
+      replace (i-i) with 0 by omega.
+      rewrite upd_Znth_same.
+      unfold upd_Znth. rewrite sublist_nil. simpl.
+      rewrite nth_first_sublist. rewrite nth_first_sublist.
+      rewrite sublist_split with (lo:=0) (mid:=i) (hi:=i+1).
+      erewrite sublist_len_1. rewrite <- app_nil_r with (l:=le_to_list le). rewrite HZNTH. simpl.
+      rewrite app_nil_r. rewrite <- app_assoc. simpl. cancel.
+      rewrite le_to_list_length. unfold n in H0. simpl in H0. rewrite H0. rewrite Fanout_eq.
+      replace (Z.of_nat 15) with 15. omega. simpl. auto. omega.
+      rewrite le_to_list_length. unfold n in H0. simpl in H0. rewrite H0. rewrite Fanout_eq.
+      replace (Z.of_nat 15) with 15. omega. simpl. auto.
+      rewrite Zlength_app. rewrite le_to_list_length. rewrite numKeys_nth_first.
+      rewrite Z2Nat.id. omega. 
+      omega. omega.
+      omega. omega.
+      rewrite le_to_list_length. rewrite numKeys_nth_first.
+      rewrite Z2Nat.id. omega.
+      omega. omega.
+      omega. omega.
+      rewrite le_to_list_length. rewrite numKeys_nth_first. rewrite Z2Nat.id. omega. omega.
+      omega.
+      rewrite Zlength_app. rewrite le_to_list_length. rewrite numKeys_nth_first. rewrite Z2Nat.id.
+      omega. omega. omega. }
+    Intros allent_end.
+    forward.                    (* t'24=entry->key *)
+    rewrite HK. unfold key_repr.
+
+    assert(FRIRANGE: (0 <= fri < 16)%nat).
+    { simpl in INRANGE. rewrite Fanout_eq in INRANGE. split. omega.
+      replace (Z.of_nat 15) with 15 in INRANGE.
+      apply Nat2Z.inj_lt. destruct INRANGE. eapply Z.le_lt_trans with (m:=15). rep_omega.
+      simpl. omega. simpl. auto. }
+    rewrite ENTRY in HEVR. simpl in HEVR. inv HEVR.
+
+    Opaque Znth.
+    forward.                    (* allEntries[tgtIdx]->key = t'24 *)
+    forward.                    (* t'23=entry->ptr.record *)
+    forward.                    (* allEntries[tgtIdx]->ptr.record = t'23 *)
+    assert(0 <= Z.of_nat fri < Zlength (le_to_list (nth_first_le le (Z.to_nat (Z.of_nat fri))) ++ allent_end)).
+    { split. omega. rewrite Zlength_app. rewrite le_to_list_length.
+      rewrite numKeys_nth_first. rewrite Z2Nat.id. rewrite Zlength_correct.
+      rewrite H3. rewrite Nat2Z.id.
+      assert(Z.of_nat(Fanout + 1 - fri) > 0).
+      { rewrite Fanout_eq. simpl in INRANGE. rewrite Nat2Z.inj_sub.
+        simpl. omega. rewrite Fanout_eq in INRANGE. simpl in INRANGE. omega. }
+      omega. omega.
+      rewrite Nat2Z.id. unfold n in H0. simpl in H0. rewrite H0. rewrite Fanout_eq. omega. }
+    rewrite upd_Znth_twice by auto. rewrite upd_Znth_same by auto.
+    deadvars!.
+    assert(FRILENGTH: Zlength (le_to_list (nth_first_le le (Z.to_nat (Z.of_nat fri)))) = Z.of_nat fri).
+    { rewrite le_to_list_length. rewrite numKeys_nth_first. rewrite Nat2Z.id. auto.
+      rewrite Nat2Z.id. unfold n in H0. simpl in H0. rewrite H0. simpl in INRANGE. omega. }
+    unfold upd_Znth. rewrite sublist_app1 by (try rep_omega; rewrite FRILENGTH; rep_omega).
+    rewrite sublist_same by (try rep_omega; rewrite FRILENGTH; rep_omega).
+    rewrite sublist_app2 by (rewrite FRILENGTH; rep_omega).
+    repeat rewrite FRILENGTH.
+    replace (Z.of_nat fri + 1 - Z.of_nat fri) with 1 by rep_omega. rewrite Zlength_app.
+    rewrite FRILENGTH.
+    replace (Z.of_nat fri + Zlength allent_end - Z.of_nat fri) with (Zlength allent_end) by rep_omega.
+
+    forward_for_simple_bound (Z.of_nat(Fanout)) ( EX i:Z, EX ent_end:list (val * (val+val)), PROP(Z.of_nat fri <= i <= Z.of_nat Fanout; length ent_end = (Fanout - Z.to_nat(i))%nat) LOCAL(temp _newNode vnewnode; temp _tgtIdx (Vint (Int.repr (Z.of_nat fri))); lvar _allEntries (tarray tentry 16) v_allEntries; temp _node nval; temp _entry pe) SEP(mem_mgr gv; btnode_rep nleft; btnode_rep (empty_node false false Last vnewnode);data_at Ews tentry (Vint (Int.repr (k_ k)), inl (getval ce)) pe; data_at Tsh (tarray tentry 16) (le_to_list (nth_first_le le (Z.to_nat (Z.of_nat fri))) ++ (Vint (Int.repr (k_ k)), inl (getval ce)) :: le_to_list(suble (fri) (Z.to_nat i) le) ++ ent_end) v_allEntries; entry_rep(keychild val ke ce)))%assert.
+
+    { simpl in INRANGE. rewrite Fanout_eq in INRANGE.
+      replace (Z.of_nat 15) with 15 in INRANGE.
+      rewrite Fanout_eq. simpl. rep_omega. simpl. auto. }
+    abbreviate_semax.
+    {                           (* second loop *)
+      forward.                  (* i=tgtidx *)
+      Exists (Z.of_nat(fri)). Exists ( sublist 1 (Zlength allent_end) allent_end).
+      entailer!.
+      simpl in INRANGE. split3; try rep_omega.
+      { clear -H3 INRANGE. destruct allent_end.
+        - simpl in H3. rewrite Nat2Z.id in H3.
+          assert((fri <= Fanout)%nat). apply Nat2Z.inj_le. omega. omega.
+        - rewrite sublist_1_cons. rewrite Zlength_cons. rewrite Zsuccminusone.
+          rewrite sublist_same; auto. simpl in H3. omega. }
+      rewrite Nat2Z.id. rewrite suble_nil. cancel. }
+    {                           (* loop body *)
+      rewrite unfold_btnode_rep with (n:=nleft). unfold nleft.
+      rename ent_end into x.
+      Intros ent_end.
+      assert(HENTRY: exists e, nth_entry_le (Z.to_nat i) le = Some e).
+      { apply nth_entry_le_in_range. simpl in H0. rewrite H0. apply Nat2Z.inj_lt.
+        rewrite Z2Nat.id. omega. omega. }
+      destruct HENTRY as [ei HENTRY].
+      assert (HEI: exists ki ci, ei = keychild val ki ci).
+      { eapply integrity_nth. eauto. simpl. auto. eauto. }
+      destruct HEI as [ki [ci HEI]]. subst ei.
+      assert_PROP(isptr (getval ci)).
+      { apply le_iter_sepcon_split in HENTRY. rewrite HENTRY. simpl entry_rep. entailer!. }
+      rename H9 into CIPTR.
+      rename H7 into IRANGE.
+      assert(HZNTH: forall ent_end, Znth (d:=(Vundef,inl Vundef)) i (le_to_list le ++ ent_end) = entry_val_rep (keychild val ki ci)).
+      { intros. rewrite <- Z2Nat.id with (n:=i). apply Znth_to_list. auto. omega. }
+      assert(HIRANGE: (0 <= i < 15)).
+      { split. rep_omega. rewrite Fanout_eq in H6. simpl in H6. rep_omega. }
+      forward.                  (* t'22=node->entries[i].key *)
+      { entailer!. rewrite HZNTH. simpl; auto. }
+      rewrite HZNTH. simpl.
+      Opaque Znth.
+      forward.                  (* allEntries[i+1].key=t'26 *)
+      forward.                  (* t'21=node->entries[i].ptr.record *)
+      { rewrite HZNTH. entailer!. }
+      rewrite HZNTH. simpl.
+      forward.                  (* allEntries[i+1]->ptr.record=t'21 *)
+      entailer!.
+      assert(XEMP: Zlength x > 0).
+      { destruct x. clear -H8 HIRANGE. rewrite Fanout_eq in H8.
+        apply eq_sym in H8. apply NPeano.Nat.sub_0_le in H8. apply inj_le in H8.
+        simpl in H8. rewrite Z2Nat.id in H8. rep_omega. omega.
+        rewrite Zlength_cons. rep_omega. }
+      Exists (sublist 1 (Zlength x) x). entailer!.
+      { clear -IRANGE H8 XEMP.
+        destruct x.
+        - rewrite Zlength_nil in XEMP. omega.
+        - rewrite sublist_1_cons. rewrite Zlength_cons. rewrite Zsuccminusone.
+          rewrite sublist_same by omega. simpl in H8. rewrite Z2Nat.inj_add by omega.
+          simpl. omega. }
+      assert(INUM: (Z.to_nat i <= numKeys_le le)%nat).
+      { unfold n  in H0. simpl in H0. rewrite H0. clear -HIRANGE.
+        rewrite Fanout_eq. destruct HIRANGE. apply Z2Nat.inj_lt in H0.
+        simpl in H0. omega. auto. omega. }
+      rewrite unfold_btnode_rep with (n:=nleft). unfold nleft. Exists ent_end. cancel.
+      rewrite Nat2Z.id.
+      rewrite upd_Znth_twice.
+      (* rewrite upd_Znth_app2. *)
+      rewrite upd_Znth_same.
+      assert((upd_Znth (i + 1) (le_to_list (nth_first_le le fri) ++ (Vint (Int.repr (k_ k)), inl (getval ce)) :: le_to_list (suble (fri) ((Z.to_nat i)) le) ++ x) (key_repr ki, inl (getval ci))) = (le_to_list (nth_first_le le fri) ++ (Vint (Int.repr (k_ k)), inl (getval ce)) :: le_to_list (suble (fri) ((Z.to_nat (i + 1))) le) ++ sublist 1 (Zlength x) x)).
+      { rewrite upd_Znth_app2. rewrite le_to_list_length. rewrite numKeys_nth_first.
+        change (?A::?B) with ([A]++B).
+        rewrite upd_Znth_app2. simpl. rewrite Zlength_cons. simpl.
+        rewrite upd_Znth_app2. rewrite le_to_list_length.
+        assert(i + 1 - Z.of_nat fri - 1 - Z.of_nat (numKeys_le (suble (fri) ((Z.to_nat i)) le)) = 0).
+        { rewrite numKeys_suble. simpl.
+          rewrite Nat2Z.inj_sub. rewrite Z2Nat.id. omega. omega.
+          rep_omega.
+          split. assert(fri <= Z.to_nat i)%nat.
+          rep_omega. omega.
+          simpl in H0. rewrite H0. clear -H6 HIRANGE. destruct H6.
+          rewrite Z2Nat.inj_lt in H0. rewrite Nat2Z.id in H0. omega.
+          omega. rep_omega. }
+        rewrite H18.
+        rewrite upd_Znth0.
+        assert(le_to_list (suble (fri) ((Z.to_nat i)) le) ++ [(key_repr ki, (inl (getval ci)):(val+val))] = le_to_list (suble (fri) ((Z.to_nat (i + 1))) le)).
+        { rewrite Z2Nat.inj_add. simpl. rewrite NPeano.Nat.add_1_r.
+          rewrite suble_increase with (e:=keychild val ki ci).
+          rewrite le_to_list_app. simpl. auto.
+          split. destruct IRANGE. clear -H19 HIRANGE. rewrite Nat2Z.inj_le. rewrite Z2Nat.id. auto.
+          omega.
+          simpl in H0. rewrite H0. apply Nat2Z.inj_lt.
+          rewrite Z2Nat.id. omega. omega.
+          auto. omega. omega. }
+        rewrite <- H19. rewrite <- app_assoc. simpl. auto.
+        
+        assert(Z.to_nat i < Z.to_nat (Z.of_nat Fanout))%nat. 
+        rewrite Nat2Z.id. apply Nat2Z.inj_lt. rewrite Z2Nat.id. omega. omega.
+        rewrite le_to_list_length. rewrite numKeys_suble. rep_omega.
+        simpl in H0. rewrite H0. split. apply Nat2Z.inj_le. rewrite Z2Nat.id. omega. omega.
+        apply Nat2Z.inj_le. rewrite Z2Nat.id. omega. omega.
+        rewrite Zlength_cons. simpl.
+        rewrite Zlength_app.
+        rewrite le_to_list_length. rewrite numKeys_suble.
+        rewrite Zlength_correct. rewrite H8.
+        split. omega. rep_omega.
+        simpl in H0. rewrite H0. split. apply Nat2Z.inj_le. rewrite Z2Nat.id. omega. omega.
+        apply Nat2Z.inj_le. rewrite Z2Nat.id. omega. omega.
+        simpl in H0. rewrite H0. apply Nat2Z.inj_le. omega.
+        rewrite Zlength_cons. rewrite Zlength_app. rewrite le_to_list_length. rewrite le_to_list_length.
+        rewrite numKeys_nth_first. rewrite numKeys_suble. split. omega.
+        rep_omega.
+        simpl in H0. rewrite H0. split. apply Nat2Z.inj_le. rewrite Z2Nat.id. omega. omega.
+        apply Nat2Z.inj_le. rewrite Z2Nat.id. omega. omega.
+        simpl in H0. rewrite H0. apply Nat2Z.inj_le. omega.
+      }
+      rewrite H18. simpl. cancel.
+      rewrite Zlength_app. rewrite Zlength_cons. rewrite le_to_list_length.
+      rewrite numKeys_nth_first. rewrite Zlength_app. rewrite le_to_list_length.
+      rewrite numKeys_suble. split. omega. rep_omega.
+      simpl in H0. rewrite H0. split. apply Nat2Z.inj_le. rewrite Z2Nat.id. omega. omega.
+        apply Nat2Z.inj_le. rewrite Z2Nat.id. omega. omega.
+      simpl in H0. rewrite H0. apply Nat2Z.inj_le. omega.
+      rewrite Zlength_app. rewrite Zlength_cons. rewrite Zlength_app.
+      rewrite le_to_list_length. rewrite le_to_list_length.
+      rewrite numKeys_nth_first. rewrite numKeys_suble. split. omega. rep_omega.
+      simpl in H0. rewrite H0. split. apply Nat2Z.inj_le. rewrite Z2Nat.id. omega. omega.
+        apply Nat2Z.inj_le. rewrite Z2Nat.id. omega. omega.
+      simpl in H0. rewrite H0. apply Nat2Z.inj_le. omega.
+    } 
+    eapply splitnode_main_ifelse_part2_proof; try eassumption.
+Qed.
